security-monitor/src/confidential_flow/handlers/symmetrical_multiprocessing/sfence_vma_asid.rs
@@ -12,6 +12,7 @@ use crate::core::control_data::{
 /// Handles a request from one confidential hart to execute sfence.vma instruction on remote confidential harts. It represents an inter hart
 /// request.
 #[derive(Clone, PartialEq)]
+#[rr::skip]
 pub struct RemoteSfenceVmaAsid {
     ipi: Ipi,
     _start_address: usize,
