verification/theories/page_allocator/page.v
@@ -1,4 +1,5 @@
 From refinedrust Require Import typing.
+From rrstd.cmp.theories Require Import ordering.
 From ace.theories.base Require Import base.
 
 (** * Extra theories for page sizes and pages *)
@@ -17,17 +18,19 @@ Global Instance page_size_inh : Inhabited page_size.
 Proof. exact (populate Size4KiB). Qed.
 Global Instance page_size_eqdec : EqDecision page_size.
 Proof. solve_decision. Defined.
+Definition page_size_variant (a : page_size) : Z :=
+  match a with
+  | Size4KiB => 0
+  | Size16KiB => 1
+  | Size2MiB => 2
+  | Size1GiB => 3
+  | Size512GiB => 4
+  | Size128TiB => 5
+  end
+.
 Global Instance page_size_countable : Countable page_size.
 Proof.
-  refine (inj_countable (λ sz,
-    match sz with
-    | Size4KiB => 0
-    | Size16KiB => 1
-    | Size2MiB => 2
-    | Size1GiB => 3
-    | Size512GiB => 4
-    | Size128TiB => 5
-    end)
+  refine (inj_countable (λ a, Z.to_nat (page_size_variant a))
     (λ a,
     match a with
     | 0 => Some Size4KiB
@@ -37,12 +40,70 @@ Proof.
     | 4 => Some Size512GiB
     | 5 => Some Size128TiB
     | _ => None
-    end) _).
+    end%nat) _).
   intros []; naive_solver.
 Qed.
 
+Global Instance page_size_variant_inj :
+  Inj (=) (=) (page_size_variant).
+Proof.
+  intros sz1 sz2.
+  destruct sz1, sz2; done.
+Qed.
+
+Definition page_size_cmp (a b : page_size) : ordering :=
+  Z.cmp (page_size_variant a) (page_size_variant b).
+Arguments page_size_cmp : simpl never.
+
+Definition page_size_eq (a b : page_size) : bool :=
+  bool_decide (a = b).
+
+Global Instance page_size_eq_correct : CorrectEq page_size_eq.
+Proof.
+  unfold page_size_eq.
+  econstructor.
+  - intros ?. naive_solver.
+  - intros ??. naive_solver.
+  - intros ???. naive_solver.
+Qed.
+Global Instance page_size_cmp_correct : CorrectOrd page_size_eq page_size_cmp.
+Proof.
+  unfold page_size_eq, page_size_cmp.
+  econstructor.
+  - apply _.
+  - intros ??. solve_goal.
+  - intros ???. solve_goal.
+  - intros ???. solve_goal.
+  - solve_goal.
+  - solve_goal.
+Qed.
+
+Notation "a '<ₚ' b" := (a <o{page_size_cmp} b) (at level 50).
+Notation "a '=ₚ' b" := (a =o{page_size_cmp} b) (at level 50).
+Notation "a '>ₚ' b" := (a >o{page_size_cmp} b) (at level 50).
+Notation "a '≤ₚ' b" := (a ≤o{page_size_cmp} b) (at level 60).
+Notation "a '≥ₚ' b" := (a ≥o{page_size_cmp} b) (at level 50).
+
+Lemma page_size_le_max p :
+  p ≤ₚ Size128TiB.
+Proof.
+  unfold ord_le.
+  destruct p; last (by right); left.
+  all: apply Z.cmp_less_iff.
+  all: simpl; lia.
+Qed.
+Lemma page_size_le_min p :
+  Size4KiB ≤ₚ p.
+Proof.
+  unfold ord_le.
+  destruct p; first (by right); left.
+  all: apply Z.cmp_less_iff.
+  all: simpl; lia.
+Qed.
+
+
 (** Number of 64-bit machine words in a page size *)
-Definition page_size_in_words_nat (sz : page_size) : nat :=
+Definition page_size_in_words_nat_def (sz : page_size) : nat :=
   match sz with
   | Size4KiB => 512
   | Size16KiB => 4 * 512
@@ -51,11 +112,14 @@ Definition page_size_in_words_nat (sz : page_size) : nat :=
   | Size512GiB => 512 * 512 * 512 * 512
   | Size128TiB => 512 * 512 * 512 * 512 * 256
   end.
+Definition page_size_in_words_nat_aux : seal (page_size_in_words_nat_def). Proof. by econstructor. Qed.
+Definition page_size_in_words_nat := page_size_in_words_nat_aux.(unseal).
+Definition page_size_in_words_nat_unfold : page_size_in_words_nat = page_size_in_words_nat_def := page_size_in_words_nat_aux.(seal_eq).
 
 Definition page_size_in_bytes_nat (sz : page_size) : nat :=
   bytes_per_addr * page_size_in_words_nat sz.
-Definition page_size_in_bytes_Z (sz : page_size) : Z :=
-  page_size_in_bytes_nat sz.
+Notation page_size_in_bytes_Z sz :=
+  (Z.of_nat (page_size_in_bytes_nat sz)).
 
 Lemma page_size_in_bytes_div_8 sz :
   (8 | page_size_in_bytes_nat sz).
@@ -67,7 +131,7 @@ Qed.
 Lemma page_size_in_words_nat_ge sz :
   page_size_in_words_nat sz ≥ 512.
 Proof.
-  unfold page_size_in_words_nat.
+  rewrite page_size_in_words_nat_unfold /page_size_in_words_nat_def.
   destruct sz; lia.
 Qed.
 Lemma page_size_in_bytes_nat_ge sz :
@@ -77,6 +141,104 @@ Proof.
   rewrite bytes_per_addr_eq.
   specialize (page_size_in_words_nat_ge sz).
   lia.
+Qed.
+Lemma page_size_in_bytes_nat_in_usize sz :
+  (Z.of_nat $ page_size_in_bytes_nat sz) ∈ usize.
+Proof.
+  rewrite /page_size_in_bytes_nat page_size_in_words_nat_unfold /page_size_in_words_nat_def.
+  rewrite bytes_per_addr_eq.
+  split.
+  all: unsafe_unfold_common_caesium_defs.
+  all: unfold it_signed, it_byte_size_log, bytes_per_addr_log.
+  all: destruct sz; try lia.
+Qed.
+Lemma page_size_in_bytes_Z_in_usize sz :
+  (page_size_in_bytes_Z sz) ∈ usize.
+Proof.
+  apply page_size_in_bytes_nat_in_usize.
+Qed.
+
+Lemma page_size_in_words_nat_mono sz1 sz2 :
+  page_size_variant sz1 < page_size_variant sz2 →
+  page_size_in_words_nat sz1 < page_size_in_words_nat sz2.
+Proof.
+  rewrite page_size_in_words_nat_unfold /page_size_in_words_nat_def.
+  unfold page_size_variant.
+  destruct sz1, sz2; lia.
+Qed.
+Lemma page_size_in_bytes_nat_mono sz1 sz2 :
+  page_size_variant sz1 < page_size_variant sz2 →
+  page_size_in_bytes_nat sz1 < page_size_in_bytes_nat sz2.
+Proof.
+  unfold page_size_in_bytes_nat.
+  intros ?%page_size_in_words_nat_mono.
+  unfold bytes_per_addr.
+  nia.
+Qed.
+Lemma page_size_in_bytes_Z_mono sz1 sz2 :
+  page_size_variant sz1 < page_size_variant sz2 →
+  page_size_in_bytes_Z sz1 < page_size_in_bytes_Z sz2.
+Proof.
+  unfold page_size_in_bytes_Z.
+  intros ?%page_size_in_bytes_nat_mono.
+  done.
+Qed.
+
+Lemma page_size_le_size_in_bytes sz1 sz2 :
+  sz1 ≤ₚ sz2 →
+  page_size_in_bytes_Z sz1 ≤ page_size_in_bytes_Z sz2.
+Proof.
+  intros [Hlt | Heq].
+  - apply Z.cmp_less_iff in Hlt.
+    apply page_size_in_bytes_Z_mono in Hlt. lia.
+  - apply Z.cmp_equal_iff in Heq. apply page_size_variant_inj in Heq. subst.
+    lia.
+Qed.
+Lemma page_size_in_words_nat_lt_divide sz1 sz2 :
+  sz1 <ₚ sz2 →
+  Nat.divide (page_size_in_words_nat sz1) (page_size_in_words_nat sz2).
+Proof.
+  intros Ha. apply Z.cmp_less_iff in Ha.
+  unfold page_size_in_bytes_nat.
+  destruct sz1, sz2; simpl in *; try lia.
+  all: rewrite page_size_in_words_nat_unfold /page_size_in_words_nat_def.
+  - exists 4%nat. lia.
+  - exists 512%nat. lia.
+  - exists (512 * 512)%nat. lia.
+  - exists (512 * 512 * 512)%nat. lia.
+  - exists (512 * 512 * 512 * 256)%nat. lia.
+  - exists 128%nat. lia.
+  - exists (128 * 512)%nat. lia.
+  - exists (128 * 512 * 512)%nat. lia.
+  - exists (64 * 512 * 512 * 512)%nat. lia.
+  - exists 512%nat. lia.
+  - exists (512 * 512)%nat. lia.
+  - exists (512 * 512 * 256)%nat. lia.
+  - exists (512)%nat. lia.
+  - exists (512 * 256)%nat. lia.
+  - exists (256)%nat. lia.
+Qed.
+Lemma page_size_in_words_nat_le_divide sz1 sz2 :
+  sz1 ≤ₚ sz2 →
+  Nat.divide (page_size_in_words_nat sz1) (page_size_in_words_nat sz2).
+Proof.
+  intros [Hlt | Heq].
+  - by eapply page_size_in_words_nat_lt_divide.
+  - apply Z.cmp_equal_iff in Heq.
+    apply page_size_variant_inj in Heq as <-.
+    done.
+Qed.
+
+Lemma page_size_in_bytes_nat_le_divide sz1 sz2 :
+  sz1 ≤ₚ sz2 →
+  Z.divide (page_size_in_bytes_Z sz1) (page_size_in_bytes_Z sz2).
+Proof.
+  intros Ha. unfold page_size_in_bytes_nat.
+  apply (page_size_in_words_nat_le_divide) in Ha.
+  apply Nat2Z.divide in Ha.
+  rewrite !(Nat2Z.inj_mul bytes_per_addr).
+  apply Z.mul_divide_mono_l.
+  done.
 Qed.
 
 (** The next smaller page size *)
@@ -93,6 +255,22 @@ Definition page_size_smaller (sz : page_size) : option page_size :=
 Lemma page_size_smaller_None sz :
   page_size_smaller sz = None ↔ sz = Size4KiB.
 Proof. destruct sz; done. Qed.
+Lemma page_size_smaller_page_size_variant sz sz' :
+  page_size_smaller sz = Some sz' →
+  page_size_variant sz' = page_size_variant sz - 1.
+Proof.
+  destruct sz, sz'; simpl; naive_solver.
+Qed.
+Lemma page_size_smaller_lt sz sz' :
+  page_size_smaller sz = Some sz' →
+  sz' <ₚ sz.
+Proof.
+  intros Hsmaller.
+  apply page_size_smaller_page_size_variant in Hsmaller.
+  unfold ord_lt, page_size_cmp.
+  apply Z.cmp_less_iff.
+  lia.
+Qed.
 
 (** The next larger page size *)
 Definition page_size_larger (sz : page_size) : option page_size :=
@@ -107,6 +285,22 @@ Definition page_size_larger (sz : page_size) : option page_size :=
 Lemma page_size_larger_None sz :
   page_size_larger sz = None ↔ sz = Size128TiB.
 Proof. destruct sz; done. Qed.
+Lemma page_size_larger_page_size_variant sz sz' :
+  page_size_larger sz = Some sz' →
+  page_size_variant sz' = page_size_variant sz + 1.
+Proof.
+  destruct sz, sz'; simpl; naive_solver.
+Qed.
+Lemma page_size_larger_gt sz sz' :
+  page_size_larger sz = Some sz' →
+  sz' >ₚ sz.
+Proof.
+  intros Hlarger.
+  apply page_size_larger_page_size_variant in Hlarger.
+  unfold ord_gt, page_size_cmp.
+  apply Z.cmp_greater_iff.
+  lia.
+Qed.
 
 (** Pages should be aligned to the size of the page;
   compute the log2 of this page's alignment *)
@@ -126,11 +320,98 @@ Lemma page_size_align_is_size sz :
   (page_size_align sz = page_size_in_bytes_nat sz)%nat.
 Proof.
   rewrite /page_size_align/page_size_in_bytes_nat/bytes_per_addr/bytes_per_addr_log.
+  rewrite page_size_in_words_nat_unfold.
   Local Arguments Nat.mul : simpl never.
   destruct sz; simpl; lia.
 Qed.
 
-(** The maximum address at which a page may be located (one-past-the-end address) *)
+(** Join on page sizes (maximum) *)
+Definition page_size_max (sz1 sz2 : page_size) : page_size :=
+  match sz1, sz2 with
+  | Size128TiB, _ => Size128TiB
+  | _ , Size128TiB => Size128TiB
+  | Size512GiB, _ => Size512GiB
+  | _, Size512GiB => Size512GiB
+  | Size1GiB, _ => Size1GiB
+  | _, Size1GiB => Size1GiB
+  | Size2MiB, _ => Size2MiB
+  | _, Size2MiB => Size2MiB
+  | Size16KiB, _ => Size16KiB
+  | _, Size16KiB => Size16KiB
+  | _, _ => Size4KiB
+  end.
+Global Instance page_size_join : Join page_size := page_size_max.
+
+Lemma page_size_max_ge_l sz1 sz2 :
+  sz1 ≤ₚ sz1 ⊔ sz2.
+Proof.
+  unfold ord_le.
+  destruct sz1, sz2; cbn; naive_solver.
+Qed.
+Lemma page_size_max_ge_r sz1 sz2 :
+  sz2 ≤ₚ sz1 ⊔ sz2.
+Proof.
+  unfold ord_le.
+  destruct sz1, sz2; cbn; naive_solver.
+Qed.
+Lemma page_size_max_l sz1 sz2 :
+  sz2 ≤ₚ sz1 → sz1 ⊔ sz2 = sz1.
+Proof.
+  intros [Hlt | Heq].
+  - apply Z.cmp_less_iff in Hlt. destruct sz1, sz2; simpl in *; try done.
+  - apply Z.cmp_equal_iff in Heq. destruct sz1, sz2; simpl; try done.
+Qed.
+Lemma page_size_max_r sz1 sz2 :
+  sz1 ≤ₚ sz2 → sz1 ⊔ sz2 = sz2.
+Proof.
+  intros [Hlt | Heq].
+  - apply Z.cmp_less_iff in Hlt. destruct sz1, sz2; simpl in *; try done.
+  - apply Z.cmp_equal_iff in Heq. destruct sz1, sz2; simpl; try done.
+Qed.
+
+(** Meet on page sizes (minimum) *)
+Definition page_size_min (sz1 sz2 : page_size) : page_size :=
+  match sz1, sz2 with
+  | Size4KiB, _ => Size4KiB
+  | _, Size4KiB => Size4KiB
+  | Size16KiB, _ => Size16KiB
+  | _, Size16KiB => Size16KiB
+  | Size2MiB, _ => Size2MiB
+  | _, Size2MiB => Size2MiB
+  | Size1GiB, _ => Size1GiB
+  | _, Size1GiB => Size1GiB
+  | Size512GiB, _ => Size512GiB
+  | _, Size512GiB => Size512GiB
+  |_, _ => Size128TiB
+  end.
+Global Instance page_size_meet : Meet page_size := page_size_min.
+
+Lemma page_size_min_le_l sz1 sz2 :
+  sz1 ⊓ sz2 ≤ₚ sz1.
+Proof.
+  unfold ord_le. destruct sz1, sz2; cbn; naive_solver.
+Qed.
+Lemma page_size_min_le_r sz1 sz2 :
+  sz1 ⊓ sz2 ≤ₚ sz2.
+Proof.
+  unfold ord_le. destruct sz1, sz2; cbn; naive_solver.
+Qed.
+Lemma page_size_min_l sz1 sz2 :
+  sz1 ≤ₚ sz2 → sz1 ⊓ sz2 = sz1.
+Proof.
+  intros [Hlt | Heq].
+  - apply Z.cmp_less_iff in Hlt. destruct sz1, sz2; simpl in *; try done.
+  - apply Z.cmp_equal_iff in Heq. destruct sz1, sz2; simpl in *; try done.
+Qed.
+Lemma page_size_min_r sz1 sz2 :
+  sz2 ≤ₚ sz1 → sz1 ⊓ sz2 = sz2.
+Proof.
+  intros [Hlt | Heq].
+  - apply Z.cmp_less_iff in Hlt. destruct sz1, sz2; simpl in *; try done.
+  - apply Z.cmp_equal_iff in Heq. destruct sz1, sz2; simpl in *; try done.
+Qed.
+
+(** The maximum address at which a page may be located (one-past-the-end address), limited by the page allocator implementation. *)
 (* Sealed because it is big and will slow down Coq *)
 Definition MAX_PAGE_ADDR_def : Z :=
   page_size_in_bytes_Z Size128TiB.
@@ -172,13 +453,6 @@ Qed.
 (** One-past-the-end location of this page *)
 Definition page_end_loc (p : page) : loc :=
   p.(page_loc) +ₗ (page_size_in_bytes_Z p.(page_sz)).
-
-(** Order on page sizes *)
-Definition page_size_le (p1 p2 : page_size) :=
-  page_size_in_words_nat p1 ≤ page_size_in_words_nat p2.
-Arguments page_size_le : simpl never.
-
-Infix "≤ₚ" := page_size_le (at level 50).
 
 (** Well-formedness of a page *)
 Definition page_wf (p : page) : Prop :=
@@ -226,6 +500,7 @@ Definition page_size_multiplier_log (sz : page_size) : nat :=
 Definition page_size_multiplier (sz : page_size) : nat :=
   2^(page_size_multiplier_log sz).
 
+
 (** The above is not correct for the smallest page size *)
 Definition number_of_smaller_pages (sz : page_size) : nat :=
   match page_size_smaller sz with
@@ -240,7 +515,8 @@ Proof.
   intros ->.
   destruct sz; simpl.
   all: unfold page_size_smaller; simplify_eq.
-  all: unfold page_size_in_words_nat, page_size_multiplier, page_size_multiplier_log.
+  all: rewrite page_size_in_words_nat_unfold /page_size_in_words_nat_def.
+  all: unfold page_size_multiplier, page_size_multiplier_log.
   all: cbn [Nat.pow]; lia.
 Qed.
 Lemma page_size_multiplier_size_in_bytes sz sz' :
@@ -274,7 +550,6 @@ Lemma page_size_multiplier_quot sz smaller_sz :
   page_size_multiplier sz = Z.to_nat (page_size_in_bytes_Z sz `quot` page_size_in_bytes_Z smaller_sz).
 Proof.
   intros Hsz.
-  rewrite /page_size_in_bytes_Z.
   rewrite (page_size_multiplier_size_in_bytes _ smaller_sz); last done.
   rewrite Nat.mul_comm.
   rewrite Nat2Z.inj_mul.
@@ -287,7 +562,6 @@ Lemma page_size_multiplier_quot_Z sz smaller_sz :
 Proof.
   intros ?.
   rewrite (page_size_multiplier_quot _ smaller_sz); last done.
-  rewrite /page_size_in_bytes_Z.
   rewrite Z2Nat.id; first done.
   apply Z.quot_pos.
   - specialize (page_size_in_bytes_nat_ge sz). lia.
@@ -304,20 +578,168 @@ Proof.
   all: lia.
 Qed.
 
+Lemma page_size_multiplier_ge sz :
+  page_size_multiplier sz ≥ 1.
+Proof.
+  unfold page_size_multiplier.
+  nia.
+Qed.
+
+(** States that the page is in the given memory range *)
+(* TODO unify all the memory range stuff *)
+Definition page_within_range (base_address : Z) (sz : page_size) (p : page) : Prop :=
+  (base_address ≤ p.(page_loc).2 ∧ p.(page_loc).2 + page_size_in_bytes_Z p.(page_sz) ≤ base_address + page_size_in_bytes_Z sz)%Z.
+
+Lemma page_within_range_inv base sz p :
+  page_within_range base sz p →
+  p.(page_sz) = sz →
+  p.(page_loc).2 = base.
+Proof.
+  unfold page_within_range.
+  intros [] <-.
+  lia.
+Qed.
+
+Lemma page_within_range_incl base1 base2 sz1 sz2 p :
+  base2 ≤ base1 →
+  base1 + page_size_in_bytes_Z sz1 ≤ base2 + page_size_in_bytes_Z sz2 →
+  page_within_range base1 sz1 p →
+  page_within_range base2 sz2 p.
+Proof.
+  unfold page_within_range.
+  simpl. intros ?? [].
+  split; lia.
+Qed.
+
+Lemma page_within_range_sz_base_inj p sz base1 base2 :
+  p.(page_sz) = sz →
+  page_within_range base1 sz p →
+  page_within_range base2 sz p →
+  base1 = base2.
+Proof.
+  unfold page_within_range.
+  intros <-.
+  lia.
+Qed.
+
+Global Arguments page_within_range : simpl never.
+Global Typeclasses Opaque page_within_range.
+
+
+
 (** Divide a page into pages of the next smaller page size *)
 (** Relational specification *)
 Definition subdivided_pages (p : page) (ps : list page) : Prop :=
-  let smaller_sz :=
-    match page_size_smaller p.(page_sz) with
-    | None => p.(page_sz)
-    | Some sz' => sz'
-    end
-  in
+  let smaller_sz := default p.(page_sz) (page_size_smaller p.(page_sz)) in
   let num_pages := page_size_multiplier p.(page_sz) in
   length ps = num_pages ∧
   (∀ (i : nat) p', ps !! i = Some p' →
     p'.(page_loc) = p.(page_loc) offset{usize}ₗ (i * page_size_in_words_nat smaller_sz) ∧
     p'.(page_sz) = smaller_sz).
+
+Global Arguments subdivided_pages : simpl never.
+Global Typeclasses Opaque subdivided_pages.
+
+Lemma subdivided_pages_lookup_size_lt i p ps p' sz' :
+  page_size_smaller p.(page_sz) = Some sz' →
+  subdivided_pages p ps →
+  ps !! i = Some p' →
+  page_sz p' = sz'.
+Proof.
+  unfold subdivided_pages.
+  intros -> [Ha Hb] Hlook.
+  apply Hb in Hlook. simpl in Hlook.
+  destruct Hlook; done.
+Qed.
+Lemma subdivided_pages_lookup_size_le i p ps p' :
+  subdivided_pages p ps →
+  ps !! i = Some p' →
+  page_sz p' ≤ₚ page_sz p.
+Proof.
+  unfold subdivided_pages.
+  intros [Ha Hb] Hlook.
+  apply Hb in Hlook. destruct Hlook as [? ->].
+  destruct (page_size_smaller p.(page_sz)) eqn:Heq.
+  - eapply page_size_smaller_lt in Heq. left. done.
+  - simpl. right.
+    apply Z.cmp_equal_iff. done.
+Qed.
+
+Lemma subdivided_pages_lookup_base_address (i : nat) p ps p' sz' :
+  page_size_smaller p.(page_sz) = Some sz' →
+  subdivided_pages p ps →
+  ps !! i = Some p' →
+  (page_loc p').2 = p.(page_loc).2 + (i * page_size_in_bytes_nat sz').
+Proof.
+  unfold subdivided_pages.
+  intros -> [Ha Hb] Hlook.
+  apply Hb in Hlook. simpl in Hlook.
+  destruct Hlook as [-> _].
+  unfold offset_loc; simpl.
+  rewrite /page_size_in_bytes_nat.
+  rewrite bytes_per_int_usize.
+  lia.
+Qed.
+
+Lemma subdivided_pages_length p ps :
+  subdivided_pages p ps →
+  length ps = page_size_multiplier p.(page_sz).
+Proof.
+  intros [Ha _]. done.
+Qed.
+
+Lemma subdivided_pages_page_within_range (i : nat) p ps p' :
+  page_size_smaller p.(page_sz) = Some p'.(page_sz) →
+  subdivided_pages p ps →
+  ps !! i = Some p' →
+  page_within_range (p.(page_loc).2 + i * page_size_in_bytes_Z p'.(page_sz)) p'.(page_sz) p'.
+Proof.
+  intros ? Hsubdivided Hlook.
+  opose proof (subdivided_pages_lookup_base_address i _ _ _ _ _ Hsubdivided _) as Hl.
+  { done. }
+  { done. }
+  split; simpl; lia.
+Qed.
+
+Lemma subdivided_pages_page_within_range' i p ps p' sz base :
+  page_size_smaller sz = Some p'.(page_sz) →
+  subdivided_pages p ps →
+  ps !! i = Some p' →
+  base = p.(page_loc).2 →
+  sz = p.(page_sz) →
+  page_within_range base sz p'.
+Proof.
+  intros Hsmaller Hsubdivided Hlook -> ->.
+
+  specialize (subdivided_pages_length _ _ Hsubdivided) as Hlen.
+  opose proof (lookup_lt_Some _ _ _ Hlook) as ?.
+
+  eapply page_within_range_incl; first last.
+  { eapply subdivided_pages_page_within_range; done. }
+  { opose proof (page_size_multiplier_size_in_bytes p.(page_sz) p'.(page_sz) _) as Heq.
+    { rewrite Hsmaller//. }
+    rewrite Heq.
+    nia. }
+  { lia. }
+Qed.
+
+Lemma subdivided_pages_lookup_inv p sz base ps p' (i : nat) (j : Z) :
+  page_size_smaller p.(page_sz) = Some sz →
+  subdivided_pages p ps →
+  ps !! i = Some p' →
+  p'.(page_sz) = sz →
+  base = p.(page_loc).2 →
+  page_within_range (base + j * page_size_in_bytes_Z sz) sz p' →
+  i = Z.to_nat j.
+Proof.
+  intros Hsmaller Hsub Hlook <- -> Hran.
+  eapply subdivided_pages_page_within_range in Hsub; [ | done | done].
+
+  opose proof (page_within_range_sz_base_inj _ _ _ _ _ Hran Hsub) as Heq; first done.
+  specialize (page_size_in_bytes_nat_ge p'.(page_sz)).
+  nia.
+Qed.
+
 
 (** Stronger functional specification *)
 Definition subdivide_page (p : page) : list page :=
@@ -434,6 +856,22 @@ Proof.
     rewrite /page_size_in_bytes_nat. lia.
 Qed.
 
+Lemma address_aligned_to_page_size_smaller addr sz smaller_sz :
+  addr `aligned_to` page_size_in_bytes_nat sz →
+  page_size_smaller sz = Some smaller_sz →
+  addr `aligned_to` page_size_in_bytes_nat smaller_sz.
+Proof.
+  rewrite -!page_size_align_is_size.
+  unfold page_size_align.
+  intros ? Hsmall.
+  enough ((2^page_size_align_log sz)%nat = 2^page_size_align_log smaller_sz * (2^(page_size_align_log sz - page_size_align_log smaller_sz)))%nat as Heq.
+  { eapply (base.aligned_to_mul_inv _ _ (2^(page_size_align_log sz - page_size_align_log smaller_sz))). rewrite -Heq. done. }
+  destruct sz; simpl in Hsmall; try done.
+  all: injection Hsmall as <-.
+  all: simpl.
+  all: lia.
+Qed.
+
 
 (** Lithium automation *)
 Global Instance simpl_exist_page Q :
@@ -448,4 +886,32 @@ Global Instance simpl_forall_page Q :
     Q (mk_page page_loc page_sz page_val)).
 Proof.
   intros ?. intros []. done.
+Qed.
+
+Global Instance simpl_impl_page_size_smaller sz sz' :
+  SimplImpl false (page_size_smaller sz = Some sz') (λ T, page_size_smaller sz = Some sz' → page_size_variant sz' = page_size_variant sz - 1 → T).
+Proof.
+  intros T. split.
+  - intros Ha Hsmall. specialize (page_size_smaller_page_size_variant _ _ Hsmall) as ?.
+    by apply Ha.
+  - intros Ha. intros. by apply Ha.
+Qed.
+Global Instance simpl_impl_page_size_larger sz sz' :
+  SimplImpl false (page_size_larger sz = Some sz') (λ T, page_size_larger sz = Some sz' → page_size_variant sz' = page_size_variant sz + 1 → T).
+Proof.
+  intros T. split.
+  - intros Ha Hlarge. specialize (page_size_larger_page_size_variant _ _ Hlarge) as ?.
+    by apply Ha.
+  - intros Ha. intros. by apply Ha.
+Qed.
+
+Global Instance simpl_both_page_size_smaller_none sz :
+  SimplBothRel (=) (page_size_smaller sz) None (sz = Size4KiB).
+Proof.
+  split; destruct sz; simpl; done.
+Qed.
+Global Instance simpl_both_page_size_larger_none sz :
+  SimplBothRel (=) (page_size_larger sz) None (sz = Size128TiB).
+Proof.
+  split; destruct sz; simpl; done.
 Qed.
