verification/theories/page_allocator/page_allocator.v
@@ -1,5 +1,6 @@
 From refinedrust Require Import typing.
 From refinedrust Require Import ghost_var_dfrac.
+From rrstd.cmp.theories Require Import ordering.
 From ace.theories.page_allocator Require Import page.
 
 (** * Page allocator ghost state *)
@@ -50,15 +51,38 @@ End page_allocator.
 
 (** * Page allocator invariants *)
 Inductive node_allocation_state :=
-  (** This page node is completely allocated *)
-  | PageTokenUnavailable
-  (** The page token in this node is available *)
-  | PageTokenAvailable
-  (** The page node is partially available, with a page of the given size being allocable *)
-  | PageTokenPartiallyAvailable (allocable_sz : page_size)
+(** This page node is completely allocated *)
+| PageTokenUnavailable
+(** The page token in this node is available *)
+| PageTokenAvailable
+(** The page node is partially available, with a page of the given size being allocable *)
+| PageTokenPartiallyAvailable (allocable_sz : page_size)
 .
 Global Instance node_allocation_state_eqdec : EqDecision node_allocation_state.
 Proof. solve_decision. Defined.
+Global Instance node_allocation_state_inhabited : Inhabited node_allocation_state.
+Proof. apply (populate PageTokenUnavailable). Qed.
+
+Global Instance node_allocation_state_join : Join node_allocation_state := λ s1 s2,
+  match s1, s2 with
+  | PageTokenAvailable, _ => PageTokenAvailable
+  | _, PageTokenAvailable => PageTokenAvailable
+  | PageTokenPartiallyAvailable sz1, PageTokenPartiallyAvailable sz2 =>
+      PageTokenPartiallyAvailable (sz1 ⊔ sz2)
+  | PageTokenPartiallyAvailable sz1, _ => PageTokenPartiallyAvailable sz1
+  | _, PageTokenPartiallyAvailable sz1 => PageTokenPartiallyAvailable sz1
+  | _, _ => PageTokenUnavailable
+  end.
+Global Instance node_allocation_state_meet : Meet node_allocation_state := λ s1 s2,
+  match s1, s2 with
+  | PageTokenUnavailable, _ => PageTokenUnavailable
+  | _, PageTokenUnavailable => PageTokenUnavailable
+  | PageTokenPartiallyAvailable sz1, PageTokenPartiallyAvailable sz2 =>
+      PageTokenPartiallyAvailable (sz1 ⊓ sz2)
+  | PageTokenPartiallyAvailable sz1, _ => PageTokenPartiallyAvailable sz1
+  | _, PageTokenPartiallyAvailable sz1 => PageTokenPartiallyAvailable sz1
+  | _, _ => PageTokenAvailable
+  end.
 
 (** Our logical representation of storage nodes *)
 Record page_storage_node : Type := mk_page_node {
@@ -73,6 +97,16 @@ Record page_storage_node : Type := mk_page_node {
   (* whether the child nodes have been initialized *)
   children_initialized : bool;
 }.
+Global Canonical Structure page_storage_nodeRT := directRT page_storage_node.
+
+Global Instance page_storage_node_inh : Inhabited page_storage_node.
+Proof.
+  constructor. eapply mk_page_node.
+  all: apply inhabitant.
+Qed.
+
+Definition page_node_update_state (node : page_storage_node) (new_state : node_allocation_state)  : page_storage_node :=
+  mk_page_node node.(max_node_size) node.(base_address) new_state node.(children_initialized).
 
 (** Compute the base address of a child node *)
 Definition child_base_address (parent_base_address : Z) (child_size : page_size) (child_index : Z) : Z :=
@@ -88,11 +122,56 @@ Definition page_storage_node_children_wf (parent_base_address : Z) (parent_node_
     (* Then all children are sorted *)
     (∀ (i : nat) child, children !! i = Some child →
       child.(max_node_size) = child_node_size ∧
-      child.(base_address) = child_base_address parent_base_address parent_node_size i)) ∧
+      child.(base_address) = child_base_address parent_base_address child_node_size i)) ∧
   (* If there can't be any children, there are no children *)
   (page_size_smaller parent_node_size = None →
     children = [])
 .
+Lemma page_storage_node_children_wf_child_lookup (i : nat) sz child_node_size base children child :
+  page_size_smaller sz = Some child_node_size →
+  page_storage_node_children_wf base sz children →
+  children !! i = Some child →
+  max_node_size child = child_node_size ∧
+  base_address child = child_base_address base child_node_size i.
+Proof.
+  intros Hsmaller Hchildren Hchild.
+  destruct Hchildren as [Hchildren _].
+  ospecialize (Hchildren _ _ _ _ Hchild); first done.
+  done.
+Qed.
+Lemma page_storage_node_children_wf_upd_state base sz children s :
+  page_storage_node_children_wf base sz children →
+  page_storage_node_children_wf base sz ((λ node, page_node_update_state node s) <$> children).
+Proof.
+  unfold page_storage_node_children_wf.
+  destruct (page_size_smaller sz) as [smaller_size | ] eqn:Heq.
+  - simpl. intros [Ha _]. split; last done.
+    intros child_sz [=<-] i child Hlook.
+    apply list_lookup_fmap_Some_1 in Hlook as (node & -> & Hlook).
+    ospecialize (Ha _ _ _ _ Hlook).
+    { done. }
+    destruct Ha as [<- Ha].
+    done.
+  - intros [_ Ha].
+    split; first done.
+    intros _. rewrite Ha; done.
+Qed.
+Lemma page_storage_node_children_wf_insert base sz children child' (i : nat) :
+  max_node_size child' = max_node_size (children !!! i) →
+  base_address child' = base_address (children !!! i) →
+  page_storage_node_children_wf base sz children →
+  page_storage_node_children_wf base sz (<[i := child']> children).
+Proof.
+  intros Hsz Haddr [Hwf1 Hwf2]. split.
+  - intros child_sz Hsmaller j ? Hlook.
+    apply list_lookup_insert_Some in Hlook as [(<- & -> & ?) | (? & ?)]; first last.
+    { by eapply Hwf1. }
+    rewrite Haddr Hsz.
+    opose proof (lookup_lt_is_Some_2 children i _) as (child' & ?); first done.
+    erewrite list_lookup_total_correct; last done.
+    by eapply Hwf1.
+  - intros Hnone. specialize (Hwf2 Hnone). rewrite Hwf2. done.
+Qed.
 
 (** Computes the maximum size this page node can allocate *)
 Definition page_node_can_allocate (node : page_storage_node) : option page_size :=
@@ -103,27 +182,17 @@ Definition page_node_can_allocate (node : page_storage_node) : option page_size 
   end.
 
 (** The logical invariant on a page node *)
-Definition page_storage_node_invariant
+Definition page_storage_node_invariant_case
   (node : page_storage_node)
   (max_sz : option page_size) (maybe_page_token : option page) (children : list page_storage_node) :=
-
-  (* The children, if any, are well-formed *)
-  page_storage_node_children_wf node.(base_address) node.(max_node_size) children ∧
-  (* the base address is suitably aligned *)
-  (page_size_align node.(max_node_size) | node.(base_address))%Z ∧
-
-  (* initialization of child nodes *)
-  (if node.(children_initialized) then length children = page_size_multiplier node.(max_node_size) else True) ∧
-
-  (* invariant depending on the allocation state: *)
   if decide (node.(allocation_state) = PageTokenUnavailable)
   then
       (* No allocation is possible *)
-      maybe_page_token = None ∧ max_sz = None ∧
+      maybe_page_token = None ∧ max_sz = None
 
       (* all children are unavailable *)
       (* TODO do we need this *)
-      Forall (λ child, child.(allocation_state) = PageTokenUnavailable) children
+      (*Forall (λ child, child.(allocation_state) = PageTokenUnavailable) children*)
   else if decide (node.(allocation_state) = PageTokenAvailable)
   then
       (* This node is completely available *)
@@ -134,11 +203,9 @@ Definition page_storage_node_invariant
         max_sz = Some (node.(max_node_size)) ∧
         (* the token spans the whole node *)
         token.(page_loc).2 = node.(base_address) ∧
-        token.(page_sz) = node.(max_node_size) ∧
-
+        token.(page_sz) = node.(max_node_size)
         (* all children are unavailable *)
-        (* TODO: do we need this? *)
-        Forall (λ child, child.(allocation_state) = PageTokenUnavailable) children
+        (*Forall (λ child, child.(allocation_state) = PageTokenUnavailable) children*)
   else
 
       (* This node is partially available with initialized children *)
@@ -147,6 +214,7 @@ Definition page_storage_node_invariant
       ∃ allocable_sz,
       node.(allocation_state) = PageTokenPartiallyAvailable allocable_sz ∧
       max_sz = Some allocable_sz ∧
+      allocable_sz <ₚ node.(max_node_size) ∧
 
       (* children need to be initialized *)
       node.(children_initialized) = true ∧
@@ -155,6 +223,44 @@ Definition page_storage_node_invariant
       ∃ i child,
         children !! i = Some child ∧
         page_node_can_allocate child = Some allocable_sz
+.
+
+Lemma page_storage_node_invariant_case_can_allocate node max_sz tok children :
+  page_storage_node_invariant_case node max_sz tok children →
+  page_node_can_allocate node = max_sz.
+Proof.
+  unfold page_storage_node_invariant_case, page_node_can_allocate.
+  destruct (allocation_state node) eqn:Heq; simpl; naive_solver.
+Qed.
+Lemma page_node_invariant_case_sized_bounded node max_sz tok children :
+  page_storage_node_invariant_case node max_sz tok children →
+  max_sz ≤o{option_cmp page_size_cmp} Some (max_node_size node).
+Proof.
+  unfold page_storage_node_invariant_case, page_node_can_allocate.
+  destruct (allocation_state node) eqn:Heq; simpl; solve_goal.
+Qed.
+
+Global Typeclasses Opaque page_storage_node_children_wf.
+Global Typeclasses Opaque page_storage_node_invariant_case.
+
+Global Arguments page_storage_node_children_wf : simpl never.
+Global Arguments page_storage_node_invariant_case : simpl never.
+
+
+Definition page_storage_node_invariant
+  (node : page_storage_node)
+  (max_sz : option page_size) (maybe_page_token : option page) (children : list page_storage_node) :=
+
+  (* The children, if any, are well-formed *)
+  name_hint "INV_WF" (page_storage_node_children_wf node.(base_address) node.(max_node_size) children) ∧
+  (* the base address is suitably aligned *)
+  (page_size_align node.(max_node_size) | node.(base_address))%Z ∧
+
+  (* initialization of child nodes *)
+  (name_hint "INV_INIT_CHILDREN" (if node.(children_initialized) then length children = page_size_multiplier node.(max_node_size) else children = [])) ∧
+
+  (* invariant depending on the allocation state: *)
+  name_hint "INV_CASE" (page_storage_node_invariant_case node max_sz maybe_page_token children)
 .
 
 Lemma page_storage_node_invariant_empty node_size base_address :
@@ -166,7 +272,105 @@ Proof.
   apply Nat2Z.divide. done.
 Qed.
 
-(** States that the page is in the given memory range *)
-(* TODO unify all the memory range stuff *)
-Definition page_within_range (base_address : Z) (sz : page_size) (p : page) : Prop :=
-  (base_address ≤ p.(page_loc).2 ∧ p.(page_loc).2 + page_size_in_bytes_Z p.(page_sz) < base_address + page_size_in_bytes_Z sz)%Z.
+Lemma page_storage_node_invariant_case_available_inv node max_sz maybe_tok children :
+  node.(allocation_state) = PageTokenAvailable →
+  page_storage_node_invariant_case node max_sz maybe_tok children →
+  ∃ tok, maybe_tok = Some tok ∧ max_sz = Some node.(max_node_size) ∧ tok.(page_loc).2 = node.(base_address) ∧ tok.(page_sz) = node.(max_node_size).
+Proof.
+  unfold page_storage_node_invariant_case.
+  intros ->. naive_solver.
+Qed.
+
+Global Instance page_storage_node_invariant_simpl_available node max_sz maybe_tok children `{!TCDone (node.(allocation_state) = PageTokenAvailable)} `{!IsVar max_sz} `{!IsVar maybe_tok} :
+  SimplImpl false (page_storage_node_invariant_case node max_sz maybe_tok children) (λ T,
+    page_storage_node_invariant_case node max_sz maybe_tok children →
+    max_sz = Some node.(max_node_size) →
+    ∀ tok,
+    maybe_tok = Some tok →
+    tok.(page_loc).2 = node.(base_address) →
+    tok.(page_sz) = node.(max_node_size) →
+    T).
+Proof.
+  rename select (TCDone _) into Hstate. unfold TCDone in Hstate.
+  intros T. split.
+  - intros Ha Hinv.
+    specialize (Ha Hinv).
+    move: Hinv.
+    unfold page_storage_node_invariant_case. rewrite Hstate.
+    simpl. intros (? & ? & ? & ? & ?).
+    eapply Ha; done.
+  - naive_solver.
+Qed.
+
+Lemma page_storage_node_invariant_has_token node max_sz tok children :
+  page_storage_node_invariant_case node max_sz (Some tok) children →
+  node.(allocation_state) = PageTokenAvailable ∧
+  node.(max_node_size) = tok.(page_sz) ∧
+  node.(base_address) = tok.(page_loc).2.
+Proof.
+  unfold page_storage_node_invariant_case.
+  repeat case_decide; simpl.
+  all: naive_solver.
+Qed.
+
+Lemma page_storage_node_invariant_not_available node tok children :
+  page_storage_node_invariant_case node None tok children →
+  node.(allocation_state) = PageTokenUnavailable ∧
+  tok = None.
+Proof.
+  unfold page_storage_node_invariant_case.
+  repeat case_decide; simpl.
+  all: naive_solver.
+Qed.
+
+Lemma page_storage_node_invariant_case_partially_available_inv node max_sz maybe_tok children sz :
+  node.(allocation_state) = PageTokenPartiallyAvailable sz →
+  page_storage_node_invariant_case node max_sz maybe_tok children →
+  max_sz = Some sz ∧ maybe_tok = None.
+Proof.
+  unfold page_storage_node_invariant_case.
+  intros ->. naive_solver.
+Qed.
+
+Global Instance page_storage_node_invariant_simpl_partially_available node max_sz maybe_tok children sz `{!TCDone (node.(allocation_state) = PageTokenPartiallyAvailable sz)} `{!IsVar max_sz} `{!IsVar maybe_tok} :
+  SimplImpl false (page_storage_node_invariant_case node max_sz maybe_tok children) (λ T,
+    page_storage_node_invariant_case node max_sz maybe_tok children →
+    max_sz = Some sz → maybe_tok = None →
+    T).
+Proof.
+  rename select (TCDone _) into Hstate. unfold TCDone in Hstate.
+  intros T. split.
+  - intros Ha Hinv. apply Ha.
+    + done.
+    + move: Hinv. unfold page_storage_node_invariant_case. rewrite Hstate.
+      simpl. naive_solver.
+    + move: Hinv. unfold page_storage_node_invariant_case. rewrite Hstate.
+      simpl. naive_solver.
+  - naive_solver.
+Qed.
+
+Lemma page_storage_node_invariant_case_unavailable_inv node max_sz maybe_tok children :
+  node.(allocation_state) = PageTokenUnavailable →
+  page_storage_node_invariant_case node max_sz maybe_tok children →
+  max_sz = None ∧ maybe_tok = None.
+Proof.
+  unfold page_storage_node_invariant_case.
+  intros ->. naive_solver.
+Qed.
+
+Global Instance page_storage_node_invariant_simpl_unavailable node max_sz maybe_tok children `{!TCDone (node.(allocation_state) = PageTokenUnavailable)} `{!IsVar max_sz} `{!IsVar maybe_tok} :
+  SimplImpl false (page_storage_node_invariant_case node max_sz maybe_tok children) (λ T,
+    page_storage_node_invariant_case node max_sz maybe_tok children →
+    max_sz = None → maybe_tok = None →
+    T).
+Proof.
+  rename select (TCDone _) into Hstate. unfold TCDone in Hstate.
+  intros T. split.
+  - intros Ha Hinv. apply Ha.
+    + done.
+    + move: Hinv. unfold page_storage_node_invariant_case. rewrite Hstate.
+      simpl. naive_solver.
+    + move: Hinv. unfold page_storage_node_invariant_case. rewrite Hstate.
+      simpl. naive_solver.
+  - naive_solver.
+Qed.
