verification/rust_proofs/ace/proofs/proof_core_page_allocator_allocator_PageStorageTreeNode_acquire_page_token_closure1.v
@@ -1,0 +1,27 @@
+From caesium Require Import lang notation.
+From refinedrust Require Import typing shims.
+From sm.ace.generated Require Import generated_code_ace generated_specs_ace generated_template_core_page_allocator_allocator_PageStorageTreeNode_acquire_page_token_closure1.
+
+Set Default Proof Using "Type".
+
+Section proof.
+Context `{RRGS : !refinedrustGS Σ}.
+
+Lemma core_page_allocator_allocator_PageStorageTreeNode_acquire_page_token_closure1_proof (π : thread_id) :
+  core_page_allocator_allocator_PageStorageTreeNode_acquire_page_token_closure1_lemma π.
+Proof.
+  core_page_allocator_allocator_PageStorageTreeNode_acquire_page_token_closure1_prelude.
+
+  repeat liRStep; liShow.
+
+  all: print_remaining_goal.
+  Unshelve. all: sidecond_solver.
+  Unshelve. all: sidecond_hammer.
+  { f_equiv; first done.
+    move: INV_CASE.
+    unfold page_node_can_allocate.
+    destruct (allocation_state child) eqn:Heq. 
+    all: sidecond_hammer. }
+  Unshelve. all: print_remaining_sidecond.
+Qed.
+End proof.
