verification/rust_proofs/ace/proofs/proof_core_page_allocator_allocator_PageStorageTreeNode_acquire_page_token_from_this_node.v
@@ -1,0 +1,31 @@
+From caesium Require Import lang notation.
+From refinedrust Require Import typing shims.
+From sm.ace.generated Require Import generated_code_ace generated_specs_ace generated_template_core_page_allocator_allocator_PageStorageTreeNode_acquire_page_token_from_this_node.
+
+Set Default Proof Using "Type".
+
+Section proof.
+Context `{RRGS : !refinedrustGS Σ}.
+
+Hint Unfold Z.divide : lithium_rewrite.
+
+Lemma core_page_allocator_allocator_PageStorageTreeNode_acquire_page_token_from_this_node_proof (π : thread_id) :
+  core_page_allocator_allocator_PageStorageTreeNode_acquire_page_token_from_this_node_lemma π.
+Proof.
+  core_page_allocator_allocator_PageStorageTreeNode_acquire_page_token_from_this_node_prelude.
+
+  rep <-! liRStep; liShow.
+  rep liRStep.
+  liInst Hevar (mk_page_node self.(max_node_size) self.(base_address) PageTokenUnavailable self.(children_initialized)).
+  rep liRStep.
+
+  all: print_remaining_goal.
+  Unshelve. all: sidecond_solver.
+  Unshelve. all: sidecond_hammer.
+  all: move: INV_CASE;
+    unfold page_storage_node_invariant_case;
+    rewrite Hstate/=;
+    sidecond_hammer.
+  Unshelve. all: print_remaining_sidecond.
+Qed.
+End proof.
