verification/rust_proofs/ace/proofs/proof_core_page_allocator_allocator_PageStorageTreeNode_calculate_child_index.v
@@ -1,0 +1,114 @@
+From caesium Require Import lang notation.
+From refinedrust Require Import typing shims.
+From sm.ace.generated Require Import generated_code_ace generated_specs_ace generated_template_core_page_allocator_allocator_PageStorageTreeNode_calculate_child_index.
+
+Set Default Proof Using "Type".
+
+Section proof.
+Context `{RRGS : !refinedrustGS Σ}.
+
+Lemma rem_le_a_minus_b a b z :
+  0 ≤ b →
+  0 < a →
+  Z.divide b a →
+  Z.divide b z →
+  a - b >= z mod a.
+Proof.
+  intros ? Ha [n Hmul_a] [m Hmul_z].
+  subst a z.
+  (* rewrite the modulus of multiples: (b*m) mod (b*n) = b * (m mod n) *)
+  rewrite Zmult_mod_distr_r.
+
+  opose proof (Z.mod_pos_bound m n _) as Hbound; first lia.
+  destruct Hbound as [Hge Hlt].      (* 0 <= m mod n < n *)
+
+  (* multiply the inequality chain by b *)
+  assert (0 <= b * (m mod n)) by (apply Z.mul_nonneg_nonneg; lia).
+  assert (b * (m mod n) <= b * (n - 1)).
+  { apply Z.mul_le_mono_nonneg_l; try lia. }
+
+  (* conclude: b * (m mod n) <= b*n - b *)
+  replace (b * (n - 1)) with (b*n - b) in * by lia.
+  lia.
+Qed.
+
+Lemma page_within_range_offset base off sz p child_sz :
+  (page_size_in_bytes_Z (page_sz p) | (page_loc p).2) →
+  (page_size_in_bytes_Z sz | base) →
+  page_size_smaller sz = Some child_sz →
+  p.(page_sz) ≤ₚ child_sz →
+  off = ((p.(page_loc).2 - base) `quot` page_size_in_bytes_Z child_sz) * page_size_in_bytes_Z child_sz →
+  page_within_range base sz p →
+  page_within_range (base + off) child_sz p.
+Proof.
+  set (i := ((p.(page_loc).2 - base) `quot` page_size_in_bytes_Z child_sz)).
+  intros Hal1 Hal2 Hsmaller Hle -> [Hran1 Hran2].
+  split; first lia.
+
+  assert (p.(page_loc).2 - base ≤ i * page_size_in_bytes_Z child_sz + Z.rem (p.(page_loc).2 - base) (page_size_in_bytes_Z child_sz)).
+  { subst i.
+    specialize (Z.quot_rem' ((page_loc p).2 - base) (page_size_in_bytes_Z child_sz)) as Heq.
+    rewrite {1}Heq. lia. }
+  enough (page_size_in_bytes_Z child_sz - page_size_in_bytes_Z (page_sz p) >= ((page_loc p).2 - base) `rem` page_size_in_bytes_Z child_sz) by lia.
+
+  rewrite Z.rem_mod_nonneg; [ | lia | ]; first last.
+  { specialize (page_size_in_bytes_nat_ge child_sz). lia. }
+  apply rem_le_a_minus_b.
+  - lia.
+  - specialize (page_size_in_bytes_nat_ge child_sz). lia.
+  - by apply page_size_in_bytes_nat_le_divide.
+  - apply Z.divide_sub_r.
+    + done.
+    + etrans; last apply Hal2.
+      apply page_size_in_bytes_nat_le_divide.
+      etrans; first done.
+      left. by apply page_size_smaller_lt.
+Qed.
+
+Lemma core_page_allocator_allocator_PageStorageTreeNode_calculate_child_index_proof (π : thread_id) :
+  core_page_allocator_allocator_PageStorageTreeNode_calculate_child_index_lemma π.
+Proof.
+  core_page_allocator_allocator_PageStorageTreeNode_calculate_child_index_prelude.
+
+  repeat liRStep; liShow.
+
+  all: print_remaining_goal.
+  Unshelve. all: sidecond_solver.
+  Unshelve. all: sidecond_hammer.
+  { move: Hrange; unfold page_within_range. solve_goal. }
+  { move: Hrange; unfold page_within_range; solve_goal. }
+  { simplify_eq. specialize (page_size_in_words_nat_ge child_node_sz). sidecond_hammer. }
+  { simplify_eq. specialize (page_size_in_words_nat_ge child_node_sz). sidecond_hammer. }
+  { (* compute the index *)
+    simplify_eq.
+    etrans; last apply Z.quot_pos; first done; first lia.
+    specialize (page_size_in_bytes_nat_ge child_node_sz).
+    lia. }
+  { simplify_eq.
+    specialize (page_size_in_bytes_nat_ge child_node_sz) as ?.
+    apply Z.quot_le_upper_bound; first lia.
+    nia. }
+  { simplify_eq.
+    specialize (page_size_in_bytes_nat_ge child_node_sz) as ?.
+    apply Z.quot_lt_upper_bound; [lia | lia | ].
+    opose proof (page_size_multiplier_size_in_bytes this_node_page_size child_node_sz _) as  Ha.
+    { by rewrite Hchild. }
+    rewrite -Nat2Z.inj_mul. rewrite -Ha.
+
+    destruct Hrange as [Hran1 Hran2].
+    move: Hran2. simpl.
+    specialize (page_size_in_bytes_nat_ge page_token0).
+    lia.
+  }
+  { simplify_eq.
+    eapply page_within_range_offset; simpl; [ | | done..].
+    - rewrite -page_size_align_is_size. done.
+    - eexists. done. }
+  { destruct Hsz_lt as [Hsz_lt |Hsz_eq].
+    - apply Z.cmp_less_iff in Hsz_lt. lia.
+    - apply Z.cmp_equal_iff in Hsz_eq. apply page_size_variant_inj in Hsz_eq.
+      simplify_eq. lia. }
+
+  Unshelve. all: print_remaining_sidecond.
+Qed.
+End proof.
