verification/rust_proofs/ace/proofs/proof_core_page_allocator_allocator_PageStorageTreeNode_divide_page_token_if_necessary.v
@@ -1,0 +1,196 @@
+From caesium Require Import lang notation.
+From refinedrust Require Import typing shims.
+From sm.ace.generated Require Import generated_code_ace generated_specs_ace generated_template_core_page_allocator_allocator_PageStorageTreeNode_divide_page_token_if_necessary.
+
+Set Default Proof Using "Type".
+
+Section proof.
+Context `{RRGS : !refinedrustGS Σ}.
+
+Lemma divide_page_token_neutral node sz children smaller_size :
+  page_size_smaller node.(max_node_size) = Some smaller_size →
+  page_storage_node_invariant_case node sz None children →
+  node.(allocation_state) ⊓ PageTokenPartiallyAvailable smaller_size = node.(allocation_state).
+Proof.
+  intros Hsmaller.
+  unfold page_storage_node_invariant_case.
+  destruct (allocation_state node) eqn:Heq; simpl.
+  - done.
+  - naive_solver.
+  - intros [_ (? & [= <-] & -> & Hlt & ? & ?)].
+    cbn. rewrite page_size_min_l; first done.
+    apply page_size_smaller_page_size_variant in Hsmaller.
+    apply Z.ord_lt_iff in Hlt.
+    apply Z.ord_le_iff.  lia.
+Qed.
+
+Lemma core_page_allocator_allocator_PageStorageTreeNode_divide_page_token_if_necessary_proof (π : thread_id) :
+  core_page_allocator_allocator_PageStorageTreeNode_divide_page_token_if_necessary_lemma π.
+Proof.
+  core_page_allocator_allocator_PageStorageTreeNode_divide_page_token_if_necessary_prelude.
+
+  repeat liRStep.
+  1: liInst Hevar (mk_page_node self.(max_node_size) self.(base_address) (PageTokenPartiallyAvailable smaller_size) true).
+  2: liInst Hevar self.
+  all: repeat liRStep; liShow.
+
+  all: print_remaining_goal.
+  Unshelve. all: sidecond_solver.
+  Unshelve. all: try lia.
+  all: try rename select (subdivided_pages _ _) into Hsubdivided.
+
+  all: try match type of Hsubdivided with
+      | subdivided_pages _ (?pref ++ (mk_page _ _ _) :: ?suff) =>
+          rename pref into prefix;
+          rename suff into suffix
+      end.
+  all: try (opose proof (page_storage_node_invariant_has_token _ _ _ _ INV_CASE) as Ha; simpl in Ha; destruct Ha as (? & <- & ?)).
+  all: match type of INV_WF with page_storage_node_children_wf _ _ ?c => rename c into children end.
+  all: rename select (children_initialized self = true) into Hchildren.
+  all: rewrite Hchildren in INV_INIT_CHILDREN.
+  all: try rename x'3 into child_index.
+
+
+  - right.
+    opose proof (subdivided_pages_lookup_size_lt (length prefix) _ _ _ _ _ Hsubdivided _) as Ha.
+    { simpl. done. }
+    { rewrite lookup_app.
+      rewrite lookup_ge_None_2; last lia.
+      solve_goal. }
+    solve_goal.
+  - opose proof (subdivided_pages_lookup_size_lt (length prefix) _ _ _ _ _ Hsubdivided _) as Ha.
+    { simpl. done. }
+    { rewrite lookup_app.
+      rewrite lookup_ge_None_2; last lia.
+      solve_goal. }
+    simpl in Ha. subst.
+    eapply (subdivided_pages_page_within_range' (length prefix)); solve_goal.
+  - rewrite -page_size_align_is_size.
+    eexists. done.
+  - rewrite INV_INIT_CHILDREN.
+    apply subdivided_pages_length in Hsubdivided.
+    solve_goal.
+  - (* point: prove length prefix = child_index *)
+    rename select (page_within_range _ _ _) into Hrange.
+
+    opose proof (subdivided_pages_lookup_size_lt (length prefix) _ _ _ _ _ Hsubdivided _) as Hsz.
+    { done. }
+    { rewrite lookup_app_r; last lia. rewrite Nat.sub_diag. done. }
+    simpl in Hsz. subst.
+
+    opose proof (subdivided_pages_lookup_inv _ _ _ _ _ (length prefix) _ _ Hsubdivided _ _ _ Hrange) as Heq; [solve_goal.. | ].
+    assert (child_index = Z.of_nat (length prefix)) as -> by lia.
+
+    odestruct (lookup_lt_is_Some_2 children (length prefix) _) as (child & Hchild).
+    { lia. }
+    opose proof (page_storage_node_children_wf_child_lookup (length prefix) _ _ _ _ _ _ INV_WF Hchild) as [Hchild_sz Hchild_loc].
+    { done. }
+
+    apply page_within_range_inv in Hrange; last done.
+    simpl in Hrange.
+
+    rewrite lookup_total_app_r; first last.
+    { solve_goal. }
+    normalize_and_simpl_goal.
+    erewrite list_lookup_total_correct; last apply Hchild.
+    done.
+  - rename select (page_within_range _ _ _) into Hrange.
+
+    opose proof (subdivided_pages_lookup_size_lt (length prefix) _ _ _ _ _ Hsubdivided _) as Hsz.
+    { done. }
+    { rewrite lookup_app_r; last lia. rewrite Nat.sub_diag. done. }
+    simpl in Hsz. subst.
+
+    opose proof (subdivided_pages_lookup_inv _ _ _ _ _ (length prefix) _ _ Hsubdivided _ _ _ Hrange) as Heq; [solve_goal.. | ].
+    assert (child_index = Z.of_nat (length prefix)) as -> by lia.
+
+    odestruct (lookup_lt_is_Some_2 children (length prefix) _) as (child & Hchild).
+    { rewrite INV_INIT_CHILDREN. lia. }
+    opose proof (page_storage_node_children_wf_child_lookup (length prefix) _ _ _ _ _ _ INV_WF Hchild) as [Hchild_sz Hchild_loc].
+    { done. }
+
+    opose proof (subdivided_pages_lookup_base_address (length prefix) _ _ _ _ _ Hsubdivided _) as Hloc.
+    { done. }
+    { rewrite lookup_app_r; last lia. rewrite Nat.sub_diag. done. }
+
+
+    rewrite lookup_total_app_r; first last.
+    { solve_goal. }
+    normalize_and_simpl_goal.
+    erewrite list_lookup_total_correct; last apply Hchild.
+
+    rewrite Hchild_loc.
+    simpl in Hloc. rewrite Hloc.
+    rewrite /child_base_address. lia.
+  - apply subdivided_pages_length in Hsubdivided.
+    solve_goal.
+  - rename select (page_within_range _ _ _) into Hrange.
+
+    opose proof (subdivided_pages_lookup_size_lt (length prefix) _ _ _ _ _ Hsubdivided _) as Hsz.
+    { done. }
+    { rewrite lookup_app_r; last lia. rewrite Nat.sub_diag. done. }
+    simpl in Hsz. subst.
+
+    opose proof (subdivided_pages_lookup_inv _ _ _ _ _ (length prefix) _ _ Hsubdivided _ _ _ Hrange) as Heq; [solve_goal.. | ].
+    assert (child_index = Z.of_nat (length prefix)) as -> by lia.
+
+    rewrite lookup_total_app_r; first last.
+    { solve_goal. }
+    normalize_and_simpl_goal.
+    + apply list_subequiv_split.
+      { solve_goal. }
+      normalize_and_simpl_goal.
+      f_equiv. lia.
+    + normalize_and_simpl_goal.
+      odestruct (lookup_lt_is_Some_2 children (length prefix) _) as (node & ?); first lia.
+      exists node. split; first done.
+      erewrite list_lookup_total_correct; last done.
+      destruct node; done.
+  - rename select (max_node_size self = Size4KiB) into Hsz.
+    rename select (page_size_smaller _ = Some _) into Hsmaller.
+    move: Hsmaller. rewrite Hsz. done.
+  - apply subdivided_pages_length in Hsubdivided. simpl in Hsubdivided. lia.
+  - rewrite skipn_all2; last lia.
+    rewrite app_nil_r.
+    by apply page_storage_node_children_wf_upd_state.
+  - eexists. done.
+  - unfold name_hint. lia.
+  - unfold name_hint.
+    rewrite skipn_all2; last lia.
+    rewrite app_nil_r.
+    simplify_eq.
+
+    rename select (allocation_state self = _) into Hstate.
+    move: INV_CASE.
+    unfold page_storage_node_invariant_case.
+    rewrite Hstate. simpl.
+    normalize_and_simpl_goal.
+    eexists. split_and!; [done | done | | done | ].
+    { apply Z.cmp_less_iff. lia. }
+    setoid_rewrite list_lookup_fmap.
+    opose proof (lookup_lt_is_Some_2 children 0%nat _) as (child & Hchild).
+    { specialize (page_size_multiplier_ge (max_node_size self)). lia. }
+    eexists 0%nat, (page_node_update_state child PageTokenAvailable).
+    rewrite Hchild.
+    split; first done.
+    opose proof (page_storage_node_children_wf_child_lookup 0%nat _ _ _ _ _ _ INV_WF Hchild) as [Hchild_sz Hchild_loc].
+    { done. }
+    rewrite -Hchild_sz//.
+  - rename select (allocation_state self = _) into Hstate.
+    rewrite Hstate. done.
+  - eexists. done.
+  - solve_goal.
+  - solve_goal.
+  - erewrite divide_page_token_neutral; [ | done | done].
+    destruct self as [? ? state ?].
+    simpl. simpl in Hchildren. rewrite Hchildren//.
+
+  all: print_remaining_goal.
+  Unshelve. all: sidecond_solver.
+  Unshelve. all: sidecond_hammer.
+  Unshelve. all: print_remaining_sidecond.
+(*Qed.*)
+Admitted. (* admitted due to long Qed *)
+End proof.
+
+
