verification/rust_proofs/ace/proofs/proof_core_page_allocator_page_Page_T_end_address.v
@@ -17,12 +17,12 @@ Proof.
   all: print_remaining_goal.
   Unshelve. all: sidecond_solver.
   Unshelve. all: sidecond_hammer.
-  { revert select (_ < (conf_end _).2).
-    specialize (conf_end_in_usize x).
-    rewrite /page_size_in_bytes_Z /page_size_in_bytes_nat; solve_goal. }
-  { revert select (_ < (conf_end _).2).
-    specialize (conf_end_in_usize x).
-    rewrite /page_size_in_bytes_Z /page_size_in_bytes_nat; solve_goal. }
+  { revert select (_ ≤ (conf_end _).2).
+    specialize (conf_end_in_usize x0).
+    rewrite /page_size_in_bytes_nat; solve_goal. }
+  { revert select (_ ≤ (conf_end _).2).
+    specialize (conf_end_in_usize x0).
+    rewrite /page_size_in_bytes_nat; solve_goal. }
   Unshelve. all: print_remaining_sidecond.
-Admitted. (* admitted due to admit_proofs config flag *)
+Qed.
 End proof.
