verification/rust_proofs/ace/proofs/proof_core_page_allocator_page_Page_T_write.v
@@ -7,58 +7,47 @@ Set Default Proof Using "Type".
 Section proof.
 Context `{RRGS : !refinedrustGS Σ}.
 
+Global Instance bla_copy : Copyable (error_Error_ty <INST!>).
+Proof. apply _. Qed.
+
 Lemma core_page_allocator_page_Page_T_write_proof (π : thread_id) :
   core_page_allocator_page_Page_T_write_lemma π.
 Proof.
   core_page_allocator_page_Page_T_write_prelude.
 
   rep <-! liRStep; liShow.
-  { 
+  {
     rename select (offset_in_bytes `rem` 8 = 0) into Hoffset.
     apply Z.rem_divide in Hoffset; last done.
     destruct Hoffset as (off' & ->).
 
     apply_update (updateable_typed_array_access self off' (IntSynType usize)).
 
-    (*rep <-! liRStep; liShow.*)
-    rep liRStep; liShow.
-  } 
+    repeat liRStep; liShow.
+  }
   { rep liRStep; liShow. }
   { rep liRStep; liShow. }
 
   all: print_remaining_goal.
   Unshelve. all: sidecond_solver.
   Unshelve. all: sidecond_hammer.
-  { 
+  {
     revert select (_ + off' * 8 < _ + page_size_in_bytes_Z _).
-    rewrite /page_size_in_bytes_Z/page_size_in_bytes_nat.
+    rewrite /page_size_in_bytes_nat.
     rewrite bytes_per_addr_eq. nia. }
-  { rewrite /name_hint.
-    rewrite bytes_per_int_usize bytes_per_addr_eq.
-    apply Z.divide_factor_r. }
-  { rewrite /name_hint.
-    assert (off' * 8 < page_size_in_bytes_Z self0) as Hx by lia.
-    revert Hx. unfold page_size_in_bytes_Z.
+  { assert (off' * 8 < page_size_in_bytes_Z self0) as Hx by lia.
+    revert Hx.
     specialize (page_size_in_bytes_div_8 self0) as (? & ->).
     rewrite bytes_per_int_usize.
     rewrite bytes_per_addr_eq. lia. }
-  { exists (Z.to_nat off'). 
+  { exists (Z.to_nat off').
     rewrite bytes_per_int_usize bytes_per_addr_eq.
     normalize_and_simpl_goal. }
-  { rewrite /name_hint.
-    rename select (¬ _ < _ < _) into Hnlt.
-    intros []. apply Hnlt. split. { 
-      enough (bytes_per_int usize > 0) by lia. 
-      rewrite bytes_per_int_usize bytes_per_addr_eq.
-      lia. }
-    revert select (_ < (conf_end _).2).
-    unfold page_size_in_bytes_Z. lia. }
-  { rewrite /name_hint.
-    intros []. 
+  { intros [].
     rename select (offset_in_bytes `rem` 8 ≠ 0) into Hen.
     apply Hen. unfold name_hint in *.
     apply Z.rem_divide; done. }
 
   Unshelve. all: print_remaining_sidecond.
-Admitted. (* admitted due to admit_proofs config flag *)
+Qed.
 End proof.
