verification/rust_proofs/ace/proofs/proof_core_page_allocator_page_Page_core_page_allocator_page_UnAllocated_divide_closure0_call_once.v
@@ -1,0 +1,22 @@
+From caesium Require Import lang notation.
+From refinedrust Require Import typing shims.
+From sm.ace.generated Require Import generated_code_ace generated_specs_ace generated_template_core_page_allocator_page_Page_core_page_allocator_page_UnAllocated_divide_closure0_call_once.
+
+Set Default Proof Using "Type".
+
+Section proof.
+Context `{RRGS : !refinedrustGS Σ}.
+
+Lemma core_page_allocator_page_Page_core_page_allocator_page_UnAllocated_divide_closure0_call_once_proof (π : thread_id) :
+  core_page_allocator_page_Page_core_page_allocator_page_UnAllocated_divide_closure0_call_once_lemma π.
+Proof.
+  core_page_allocator_page_Page_core_page_allocator_page_UnAllocated_divide_closure0_call_once_prelude.
+
+  repeat liRStep; liShow.
+
+  all: print_remaining_goal.
+  Unshelve. all: sidecond_solver.
+  Unshelve. all: sidecond_hammer.
+  Unshelve. all: print_remaining_sidecond.
+Qed.
+End proof.
